Strenghten valid partitions to be free of empty sets.

src/dafny/utils/Partition.dfy
@@ -12,15 +12,17 @@
  * under the License.
  */
 
-// include "./MiscTypes.dfy"
-// include "./int.dfy"
-
-/** 
-  * Provides finitie automata.
-  */
+include "./SeqOfSets.dfy"
+include "./MiscTypes.dfy"
+  /** 
+    * Provides finitie automata.
+    */
 module PartitionMod {
 
-  //   import opened MiscTypes
+  import opened SeqOfSets
+  import opened MiscTypes
+
+  type ValidPartition = x: Partition | x.IsValid() witness Partition(1, [{0}])
 
   /**
     *   A partition is a list of sets but we represent them by seq to 
@@ -35,133 +37,183 @@ module PartitionMod {
       */
     ghost predicate IsValid()
     {
+      && n > 0
+      && (forall k:: 0 <= k < |elem| ==> elem[k] != {})
       && (forall k, k':: 0 <= k < k' < |elem| ==> elem[k] * elem[k'] == {})
-      && SetUnion(elem) == set q | 0 <= q < n
+      && SetU(elem) == set q {:nowarn} | 0 <= q < n
+    }
+
+    function {:tailrecursion true} SplitAllFrom(f: nat -> bool, index: nat := 0): (p': Partition)
+      requires this.IsValid()
+      requires index <= |elem|
+      decreases |elem| - index
+      ensures p'.IsValid()
+    {
+      if |elem| == index then this
+      else
+        var p1 := SplitAt(f, index);
+        //  We may add one or zero sets depending on whether splitting elem[index]
+        //  results in one empty set. If we get one set we advance to index + 1 and
+        //  if we get two we advance to index + 2
+        p1.SplitAllFrom(f, index + 1 + |p1.elem| - |elem|) 
     }
 
     /**
       *  Split a partition according to a predicate
       */
-    function {:tailrecursion true} Split(f: nat -> bool): seq<set<nat>> // (p': Partition)
+    function {:tailrecursion true} SplitAt(f: nat -> bool, index: nat): (p': Partition)
+      requires index < |elem|
       requires this.IsValid()
+        ensures p'.IsValid()
+        ensures |elem| + 1 >= |p'.elem| >= |elem|
+        ensures p'.n == n
     {
-      //  Split elem[0] according to value of f for its elements
-      if |elem| == 0 then []
-      else
-        // var setAsSeq := SetToSequence(elem[0]);
-        // elem
-        var r := SplitSet(elem[0], f);
-        [r.0, r.1] +  elem[1..]
+      //  Split elem[index] according to value of f for its elements
+      var r := SplitSet(elem[index], f);
+      assert elem[index] != {};
+      assert r.0 != {} || r.1 != {};
+      var newP := elem[..index] + [r.0, r.1] + elem[index + 1..];
+      assert (forall k, k':: 0 <= k < k' < |newP| ==> newP[k] * newP[k'] == {});
+      assert r.0 + r.1 == elem[index];
+      assert newP[index] == r.0 && newP[index + 1] == r.1;
+      calc == {
+        SetU(newP);
+        { SplitUnion2(newP, index); }
+        SetU(newP[..index] )+ newP[index] + newP[index + 1] +  SetU(newP[index + 2..]);
+        { assert newP[index] == r.0 && newP[index + 1] == r.1; }
+        SetU(newP[..index]) + r.0 + r.1 + SetU(newP[index + 2..]);
+        { assert newP[..index] == elem[..index] ;}
+        SetU(elem[..index]) + r.0 + r.1 + SetU(newP[index + 2..]);
+        { assert newP[index + 2..] == elem[index + 1..] ;}
+        SetU(elem[..index]) + r.0 + r.1 + SetU(elem[index + 1..]);
+        { assert r.0 + r.1 == elem[index]; }
+        SetU(elem[..index]) + elem[index] + SetU(elem[index + 1..]);
+        { SplitUnion1(elem, index); }
+        SetU(elem);
+      }
+      //    if one of r.0 or r.1 is empty remove it
+      if r.0 == {} then RemoveEmpty(Partition(n, newP), index)
+      else if r.1 == {} then RemoveEmpty(Partition(n, newP), index + 1)
+      else Partition(n, newP)
+    }
+
+    /**
+      * The class of a nat in {0, ..., n - 1}.
+      */
+    function GetClass(x: nat, index: nat := 0): (c: nat)
+      requires IsValid()
+      requires 0 <= x < n
+      requires index < |elem|
+      requires forall k:: 0 <= k < index ==> x !in elem[k]
+      ensures c < |elem| && x in elem[c]
+      decreases |elem| - index
+    {
+      //    This lemma ensures we will find a class index!
+      ExistsIn(this, x);
+      if x in elem[index] then index
+      else GetClass(x, index + 1)
+    }
+
+    /**
+      * Whether two nats are in the same class.
+      */
+    predicate Equiv(x: nat, y: nat)
+      requires this.IsValid()
+      requires 0 <= x < n
+      requires 0 <= y < n
+      ensures Equiv(x, y) ==> exists k:: 0 <= k < |elem| && x in elem[k] && y in elem[k]
+      ensures x == y ==> Equiv(x, y)
+    {
+      //    Prove that |p.elem|
+      NotEmpty(this);
+      assert GetClass(x) == GetClass(y) ==> x in elem[GetClass(x)] && y in elem[GetClass(y)];
+      GetClass(x) == GetClass(y)
+    }
+
+    /**
+      * Whether this refines p.
+      */
+    predicate Refines(p: Partition)
+      requires IsValid()
+      requires p.IsValid()
+      requires p.n == n
+      // ensures Refines(p) ==> |elem| >= |p.elem|
+    {
+      forall x, x':: 0 <= x < x' < n ==> (Equiv(x, x') ==> p.Equiv(x, x'))
     }
 
   }
 
-  /**
-    *   Split a set into two subsets X and Y such that X = f^-1(true) and Y = f^-1(false)
-    */
-  function SplitSet(xs: set<nat>, f: nat -> bool): (r: (set<nat>, set<nat>))
-    ensures xs == r.0 + r.1
+  function RemoveEmpty(p: Partition,  k: nat): (p': Partition)
+    requires 0 <= k < |p.elem|
+    requires p.elem[k] == {}
+    requires p.n > 0
+    requires forall k, k':: 0 <= k < k' < |p.elem| ==> p.elem[k] * p.elem[k'] == {}
+    requires SetU(p.elem) == set q {:nowarn} | 0 <= q < p.n
+    requires forall i:: 0 <= i < |p.elem| && i != k ==> p.elem[i] != {}
+    ensures p'.IsValid()
   {
-    var asSeq := SetToSequence(xs);
-    SplitSeq(asSeq, f)
+    var p1 := Partition(p.n, p.elem[..k] + p.elem[k + 1..]);
+    RemoveEmptySet(p, k);
+    p1
+
   }
 
   /**
-    *   Split a sequence of nat according to a function value f.
+    *   A valid partition cannot be empty.
     */
-  function {:tailrecursion true} SplitSeq(xs: seq<nat>, f: nat -> bool, cTrue: set<nat> := {}, cFalse: set<nat> := {}, index: nat := 0): (r: (set<nat>, set<nat>))
-    requires index <= |xs|
-    requires  forall k:: k in xs[..index] <==> k in cTrue + cFalse
-
-    ensures  forall k:: k in xs <==> k in r.0 + r.1
-
-    decreases |xs| - index
+  lemma NotEmpty(p: Partition)
+    requires p.IsValid()
+    ensures |SetU(p.elem)| > 0
+    ensures |p.elem| > 0
   {
-    if |xs| == index then (cTrue, cFalse)
-    else if f(xs[index]) then
-      //   assert forall k:: k in xs[..index] <==> k in cTrue + cFalse
-      assert xs[..index + 1] == xs[..index] + [xs[index]];
-      SplitSeq(xs, f, cTrue + {xs[index]}, cFalse, index + 1)
-    else
-      assert !f(xs[index]);
-      assert xs[..index + 1] == xs[..index] + [xs[index]];
-      SplitSeq(xs, f, cTrue, cFalse + {xs[index]}, index + 1)
+    assert { 0 } <= SetU(p.elem);
   }
 
   /**
-    *   Union of a seq of sets.
+    *   A partition p of {0, ..., n - 1} ensures that 
+    *   0 <= k < n ==> k in a class of p.
     */
-  function {:tailrecursion true} SetUnion<T>(xs: seq<set<T>>, c: set<T> := {}, index: nat := 0): (r: set<T>)
-    requires index <= |xs|
-    requires forall k:: 0 <= k < index ==> xs[k] <= c
-    requires forall e:: e in c ==> exists k:: 0 <= k < index && e in xs[k]
-
-    ensures forall k:: k in xs ==> k <= r
-    ensures forall e:: e in r ==> exists k:: 0 <= k < |xs| && e in xs[k]
-    decreases |xs| - index
+  lemma ExistsIn(p: Partition, k: nat)
+    requires p.IsValid()
+    requires 0 <= k < p.n
+    ensures exists s:: 0 <= s < |p.elem| && k in p.elem[s]
   {
-    if |xs| == index then c
-    else
-      SetUnion(xs, c + xs[index], index + 1)
-  }
-
-  /**
-    *   Intersection of a seq of sets.
-    */
-  function {:tailrecursion true} SetIntersection<T(!new)>(xs: seq<set<T>>, c: set<T> := {}, index: nat := 0): (r: set<T>)
-    requires index <= |xs|
-    requires forall k:: 0 <= k < index ==> c <= xs[k]
-    requires forall e:: e in c ==> forall k:: 0 <= k < index && e in xs[k]
-    requires forall e:: (forall k:: 0 <= k < index ==> e in xs[k]) ==> e in c
-
-    ensures forall k:: k in xs ==> r <= k
-    ensures forall e:: e in r ==> (forall k:: 0 <= k < |xs| ==> e in xs[k])
-    ensures forall e:: (forall k:: 0 <= k < |xs| ==> e in xs[k]) ==> e in r
-    decreases |xs| - index
-  {
-    if |xs| == index then c
-    else
-      SetIntersection(xs, c * xs[index], index + 1)
-  }
-
-  //  Helpers
-
-  /**
-    *   Iterate over sets. 
-    *   @link{https://leino.science/papers/krml275.html}
-    */
-  function {:tailrecursion true} SetToSequence(s: set<nat>): (r: seq<nat>)
-    ensures forall i :: i in s <==> i in r
-  {
-    if s == {} then []
-    else
-      ThereIsAMinimum(s);
-      var x :| x in s && forall y :: y in s ==> x <= y;
-      [x] + SetToSequence(s - {x})
-  }
-
-  /**
-    *   @link{https://leino.science/papers/krml275.html}
-    */
-  lemma ThereIsAMinimum(s: set<nat>)
-    requires s != {}
-    ensures exists x :: x in s && forall y :: y in s ==> x <= y
-  {
-    var x :| x in s;
-    if s == {x} {
-    } else {
-      var s' := s - {x};
-      assert s == s' + {x};
-      ThereIsAMinimum(s');
+    if !exists s:: 0 <= s < |p.elem| && k in p.elem[s] {
+      assert forall s:: 0 <= s < |p.elem| ==> k !in p.elem[s];
+      assert false;
     }
   }
 
-  method {:test} Test1() {
-    var p1 := Partition(4, [set q | 0 <= q < 4]);
-    PrintPartition(p1);
-    var p2 := p1.Split((x => x % 2 == 0));
-    PrintPartition(Partition(4, p2));
+  lemma RemoveEmptySet(p: Partition, k: nat)
+    requires 0 <= k < |p.elem|
+    requires p.elem[k] == {}
+    requires p.n > 0
+    requires forall k, k':: 0 <= k < k' < |p.elem| ==> p.elem[k] * p.elem[k'] == {}
+    requires SetU(p.elem) == set q {:nowarn} | 0 <= q < p.n
+    requires forall i:: 0 <= i < |p.elem| && i != k ==> p.elem[i] != {}
+    ensures Partition(p.n, p.elem[..k] + p.elem[k + 1..]).IsValid()
+  {
+    var p1 := Partition(p.n, p.elem[..k] + p.elem[k + 1..]);
+    NeutralEmptySet(p.elem, k);
   }
+
+  //    Some tests
+  //   method {:test} Test1() {
+  //     var p1 := Partition(4, [set q {:nowarn} | 0 <= q < 4]);
+  //     PrintPartition(p1);
+  //     var p2 := p1.SplitAllFrom((x => x % 2 == 0));
+  //     PrintPartition(p2);
+  //   }
+
+  //   method {:test} Test2() {
+  //     var p1 := Partition(20, [set q {:nowarn} | 0 <= q < 20]);
+  //     PrintPartition(p1);
+  //     var p2 := p1.SplitAllFrom((x => x % 2 == 0));
+  //     var p3 := p2.SplitAllFrom((x => x / 3 == 0));
+  //     var p4 := p3.SplitAllFrom((x => x / 4 == 0));
+  //     PrintPartition(p4);
+  //   }
 
   method {:tailrecursion true} PrintPartition(p: Partition)
   {
@@ -170,5 +222,144 @@ module PartitionMod {
       print setToSeq, "\n";
     }
   }
+
+  //    automaton
+  //    0 - a -> 1 - b -> 2
+  //    0 - b -> 3 - b -> 4
+  //    predicate is:
+  //    same enabled + s - x -> s'
+  //    s ~ s' and     s - a -> s1 and s' - a -> s1' and s1 ~ s1'
+  //    same class OK  GetClass(succ_a(s)) == GetClass(succ_a(s'));
+  /*
+  C0 = {0, 1, 3} C1 = {2, 4}
+  get tgt class of 0 in {0, 1, 3}
+  then sort according to who is equiv to 0 by succ_a(), succ_b 
+  succ_a_b(0) = (GetClass(Some(x)), None)
+
+  refine C0 = {0, 1, 3} with succ_a_b(s) == (GetClass(Some(x)), None)
+  e.g. 
+  succ_a_b(0) = (Some(1), Some(3)) -> class (Some(C0), Some(C0))
+
+  succ_a_b(1) = (None, Some(C1)) != 
+  succ_a_b(3) = (None, Some(C1)) != 
+
+  C0 refined in { 0 }, {1, 3}
+  Apply to {1, 3}
+  succ_a_b(1) = (None, C1)
+  succ_a_b(3) = (None, C1) done
+  {0}, {1, 3}, {2, 4}
+  */
+  //   method {:test} Test3()
+  //   {
+  //     var p1 := Partition(5, [set q {:nowarn} | 0 <= q < 5]);
+  //     // var p1 := Partition(5, [{0, 1, 3}, {2, 4}]);
+  //     var m: map<(nat, nat), nat> :=
+  //       map[
+  //         (0, 0) := 1,
+  //         (0, 1) := 3,
+  //         (1, 1) := 2,
+  //         (3, 1) := 4
+  //       ];
+  //     assert p1.IsValid();
+  //     assert forall k:: k in m.Values  ==> 0 <= k < p1.n;
+  //     PrintPartition(p1);
+  //     var f: ValidPair -> (nat -> (nat -> bool)) :=
+  //       (p: ValidPair) =>
+  //         ((y: nat) => ((x: nat) => succ(x, p.1, p.0) == succ(y, p.1, p.0)));
+
+  //     var pair1 := (p1, m);
+
+  //     var p2 := p1.SplitAt(f(pair1)(0), 0);
+  //     PrintPartition(p2);
+  //     // PrintPartition(pair1.0);
+  //     assert |p2.elem| > 1;
+  //     var pair2 := (p2, m);
+  //     var p3 := p2.SplitAt(f(pair2)(1), 1);
+  //     PrintPartition(p3);
+
+  //   }
+
+
+  type ValidPair = x : (Partition, map<(nat, nat), nat>) | x.0.IsValid() && (forall k:: k in x.1.Values ==> k < x.0.n)
+    witness (Partition(1, [{0}]), map[])
+
+  function succ(x: nat, m: map<(nat, nat), nat>, p: ValidPartition): (Option<nat>, Option<nat>)
+    requires forall k:: k in m.Values ==> 0 <= k < p.n
+    requires p.IsValid()
+  {
+    NotEmpty(p);
+    var s1 := if (x, 0) in m then
+                assert m[(x, 0)] in m.Values;
+                Some(p.GetClass(m[(x, 0)]))
+              else None;
+    var s2 := if (x, 1) in m then
+                assert m[(x, 1)] in m.Values;
+                Some(p.GetClass(m[(x, 1)]))
+              else None;
+    (s1, s2)
+  }
+
+  //   function foo(x: nat, p: Partition, m: map<(nat, nat), nat>): bool
+  //   {
+
+  //   }
+
+
+
+  //   lemma foo707(p: Partition, p': Partition, x: nat, y: nat)
+  //     requires p.IsValid()
+  //     requires p'.IsValid()
+  //     requires 0 <= x < p.n
+  //     requires 0 <= y < p.n
+  //     requires p.n == p'.n
+  //     requires p.Equiv(x, y)
+  //     requires p'.Equiv(x, y)
+
+
+  //   lemma foo404(p: Partition, p': Partition)
+  //     requires p.IsValid()
+  //     requires p'.IsValid()
+  //     requires p.n == p'.n
+  //     requires p.Refines(p')
+  //     // ensures forall k:: k in p.elem ==> exists k':: k' in p'.elem && k <= k'
+  //   {
+  //     NotEmpty(p);
+  //     NotEmpty(p');
+  //     assert |p'.elem| >= 1;
+
+  //     forall k | 0 <= k < |p.elem|
+  //       ensures exists k':: 0 <= k' < |p'.elem| && p.elem[k] <= p.elem[k'] {
+  //       if p.elem[k] == {} {
+  //         assert |p'.elem| >= 1;
+  //         //   assume p.elem[k] <= p'.elem[0];
+  //       } else {
+  //         //   var x :| x in p.elem[k];
+  //         //   assume x in p.elem[p.GetClass(x)];
+  //         //   assume x < p.n;
+  //         //   assume p.Equiv(x, x);
+
+  //       }
+  //       assume exists k':: 0 <= k' < |p'.elem| && p.elem[k] <= p.elem[k'];
+  //     }
+
+  //   }
+  //   lemma GetClassUnique(p: Partition, x: nat)
+  //     requires p.IsValid()
+  //     requires 0 <= x < p.n
+  //     ensures forall k:: 0 <= k < |p.elem| && k != p.GetClass(x) ==> x !in p.elem[k]
+  //   {
+  //     assume  forall k:: 0 <= k < |p.elem| && k != p.GetClass(x) ==> x !in p.elem[k];
+  //   }
+
+  //   lemma GetClassLemma(p: Partition, x: nat)
+  //     requires p.IsValid()
+  //     requires 0 <= x < p.n
+  //     requires |p.elem| > 0
+  //     ensures p.GetClass(x) < |p.elem|
+  //     ensures x in p.elem[p.GetClass(x)]
+  //   {
+  //     // NotEmpty(p);
+  //   }
+
 
 }
